---
author: "Nathaniel Hayman"
date: "010-31-2023"
output: html_document
---

1. a)
$$
\text{Assuming $X_1...X_n\sim N(\mu, \theta)$,}\\
\quad\\
\mu_1=E(X_i)=\mu;\quad\mu_2=E(X_i^2)=\text{Var}(X_i)+E(X_i)^2=\theta^2+\mu^2\\
\quad\\
\hat\mu_1=\frac{1}{n}\sum_iX_i=\bar{X};\quad\hat\mu_2=\frac{1}{n}\sum_iX_i^2\\
\quad\\
\begin{aligned}
    \mu_1&=\hat\mu_1\\
    \mu&=\bar{X}\\
    \quad\\
    \mu_2&=\hat\mu_2\\
    \theta^2+\mu^2&=\frac{1}{n}\sum_iX_i^2\\
    \theta^2+\bar X^2&=\frac{1}{n}\sum_iX_i^2\\
    \theta&=\sqrt{\frac{1}{n}\sum_iX_i^2+\bar X^2}\\
    &=\frac{1}{n}\sum_iX_i+\bar X
\end{aligned}
$$

b)
$$
\begin{aligned}
    \text{lik}(\theta)&=\prod_if(x_i|\theta)\\
    &=\prod_i\frac{1}{\sqrt{2\pi\theta}}\exp{(-\frac{1}{2\theta}(x_i-\mu)^2)}\\
    &=\sum_i\log\left[\frac{1}{\sqrt{2\pi\theta}}\exp{(-\frac{1}{2\theta}(x_i-\mu)^2)}\right]\\
    &=\sum_i\log{\frac{1}{\sqrt{2\pi\theta}}}-\frac{1}{2\theta}(x_i-\mu)^2\\
    &=n\log{\frac{1}{\sqrt{2\pi\theta}}}-\frac{1}{2\theta}\sum_i(x_i-\mu)^2\\
    \frac{d\mathscr{L}}{d\theta}&=-\frac{n}{2\theta}-\frac{1}{2\theta^2}\sum_i(x_i-\mu)^2\\
    \frac{d\mathscr{L}}{d\theta}&=0\\
    \theta&=-\frac{1}{n}\sum_i(x_i-\mu)^2\\
    \quad\\
    \text{lik}(\mu)&=\prod_if(x_i|\theta)\\
    &=n\log{\frac{1}{\sqrt{2\pi\theta}}}-\frac{1}{2\theta}\sum_i(x_i-\mu)^2\\
    &=n\log{\frac{1}{\sqrt{2\pi\theta}}}-\frac{1}{2\theta}\left[n\mu^2+\sum_ix_i^2-2\mu x_i\right]\\
    \frac{d\mathscr{L}}{d\mu}&=-\frac{1}{2\theta}\left[2n\mu^2+\sum_ix_i^2-2x_i\right]\\
    \frac{d\mathscr{L}}{d\mu}&=0\\
    2n\mu^2&=-\sum_ix_i^2-2x_i\\
    \mu&=\sqrt{\frac{-\sum_ix_i^2-2x_i}{2n}}
\end{aligned}

$$

2.
$$
X_1...X_n\sim \text{Exp}(\lambda)\\
\quad\\
\begin{aligned}
    \text{lik}(\lambda)&=\prod_i\lambda e^{-\lambda x_i}\\
    &=\sum_i\log{(\lambda e^{-\lambda x_i})}\\
    &=n\log{\lambda}-\lambda\sum_ix_i\\
    \frac{d\mathscr{L}}{d\lambda}&=\frac{n}{\lambda}-\sum_ix_i\\
    \frac{d\mathscr{L}}{d\lambda}&=0\\
    \lambda&=\frac{n}{\sum_ix_i}\\
\end{aligned}
$$

3.
a)
$$
\text{Assuming $X_1...X_n$ are iid $N(\mu, \sigma^2)$}\\
t_{n-1,\alpha/2}=t_{49,0.1}=\texttt{qt(0.9, 49)}=1.299069\\
\mu \plusmn t_{n-1,\alpha/2}\frac{S}{\sqrt{n}}=\mu \plusmn (1.299069)\frac{18}{\sqrt{50}}
$$

b) The 90% confidence interval would be wider because $L \propto MOE$

c) Yes, this is the correct interpretation

4. 
$$
\hat p \plusmn z_{\alpha/2}\sqrt{\frac{\hat p(1-\hat p)}{n}}\\
\quad\\
z_{\alpha/2}=\texttt{qnorm(0.99, 0, 1)}=2.326348\\
\hat p(1-\hat p) = 0.08(1-0.08) = 0.0736\\
\quad\\
\hat p \plusmn 0.0050203
$$
